code: Change b2w into a definition
The reifier looks for word.of_Z to determine if it should use the Z reifier or
the word one, and we want b2w to trigger the word case (in the long term it
would likely be better to rewrite the reifier to allow mixed word/Z expressions,
though, since the current code will do the wrong thing for `b2w (Z.ltb … …)`).

src/Rupicola/Lib/Core.v
@@ -754,17 +754,21 @@ Module word.
         lia.
     Qed.
 
-    Local Notation b2w b :=
+    Definition b2w (b: bool) :=
       (@word.of_Z _ word (Z.b2z b)).
 
     Lemma b2w_inj:
       forall b1 b2, b2w b1 = b2w b2 -> b1 = b2.
     Proof.
-      intros [|] [|]; simpl;
+      unfold b2w; intros [|] [|]; simpl;
         intros H%(f_equal word.unsigned);
         rewrite ?word.unsigned_of_Z_0, ?word.unsigned_of_Z_1 in H;
         cbn; congruence.
     Qed.
+
+    Lemma unsigned_b2w b:
+      word.unsigned (b2w b) = Z.b2z b.
+    Proof. apply unsigned_of_Z_b2z. Qed.
 
     Ltac compile_binop_zzw_bitwise lemma :=
       intros; cbn;
@@ -788,8 +792,6 @@ Module word.
   End __.
 End word.
 
-Notation b2w b :=
-  (word.of_Z (Z.b2z b)).
 Notation word_of_byte b :=
   (word.of_Z (Byte.byte.unsigned b)).
 Notation byte_of_word w :=
